GraphAlgorithms.v
@@ -1,0 +1,244 @@
+From Stdlib Require Import List Bool Arith Lia.
+Import ListNotations.
+
+(** Small executable graph routines over an explicit finite vertex list.
+
+    The algorithms are intentionally simple.  They are meant as verified
+    building blocks for finite automata graph criteria, not as asymptotically
+    optimal implementations. *)
+
+Section GraphAlgorithms.
+  Context {V : Type}.
+  Context (eqb : V -> V -> bool).
+  Context (eqb_sound : forall x y, eqb x y = true -> x = y).
+
+  Definition graph_edge := V -> V -> bool.
+
+  Inductive walk (edge : graph_edge) : V -> V -> Prop :=
+  | Walk_refl :
+      forall x, walk edge x x
+  | Walk_step :
+      forall x y z,
+        edge x y = true ->
+        walk edge y z ->
+        walk edge x z.
+
+  Lemma walk_trans :
+    forall edge x y z,
+      walk edge x y ->
+      walk edge y z ->
+      walk edge x z.
+  Proof.
+    intros edge x y z Hxy Hyz.
+    induction Hxy as [x| x y' z' Hedge _ IH]; auto.
+    eapply Walk_step; eauto.
+  Qed.
+
+  Fixpoint path_of_lengthb
+      (vertices : list V)
+      (edge : graph_edge)
+      (n : nat)
+      (x y : V) : bool :=
+    match n with
+    | O => eqb x y
+    | S n' =>
+        existsb
+          (fun z => edge x z && path_of_lengthb vertices edge n' z y)
+          vertices
+    end.
+
+  Fixpoint inb (x : V) (xs : list V) : bool :=
+    match xs with
+    | [] => false
+    | y :: ys => eqb x y || inb x ys
+    end.
+
+  Definition successors
+      (vertices : list V)
+      (edge : graph_edge)
+      (x : V) : list V :=
+    filter (edge x) vertices.
+
+  Fixpoint add_fresh
+      (xs seen todo : list V) : list V :=
+    match xs with
+    | [] => todo
+    | x :: xs' =>
+        let already_seen := inb x seen || inb x todo in
+        add_fresh xs' seen (if already_seen then todo else x :: todo)
+    end.
+
+  Fixpoint dfs
+      (vertices : list V)
+      (edge : graph_edge)
+      (fuel : nat)
+      (seen todo : list V)
+      (target : V) : bool :=
+    match fuel with
+    | O => false
+    | S fuel' =>
+        match todo with
+        | [] => false
+        | x :: todo' =>
+            if inb x seen then dfs vertices edge fuel' seen todo' target
+            else if eqb x target then true
+            else
+              dfs
+                vertices
+                edge
+                fuel'
+                (x :: seen)
+                (add_fresh (successors vertices edge x) (x :: seen) todo')
+                target
+        end
+    end.
+
+  Definition reachb
+      (vertices : list V)
+      (edge : graph_edge)
+      (fuel : nat)
+      (x y : V) : bool :=
+    dfs vertices edge (S fuel) [] [x] y.
+
+  Definition connectedb
+      (vertices : list V)
+      (edge : graph_edge)
+      (fuel : nat)
+      (x y : V) : bool :=
+    reachb vertices edge fuel x y && reachb vertices edge fuel y x.
+
+  Fixpoint max_nats (xs : list nat) : nat :=
+    match xs with
+    | [] => 0
+    | x :: xs' => Nat.max x (max_nats xs')
+    end.
+
+  Fixpoint max_special_path_from
+      (vertices : list V)
+      (edge special : graph_edge)
+      (fuel : nat)
+      (x : V) : nat :=
+    match fuel with
+    | O => 0
+    | S fuel' =>
+        max_nats
+          (map
+             (fun y =>
+                if edge x y
+                then
+                  (if special x y then 1 else 0)
+                  + max_special_path_from vertices edge special fuel' y
+                else 0)
+             vertices)
+    end.
+
+  Definition max_special_edges
+      (vertices : list V)
+      (edge special : graph_edge)
+      (fuel : nat) : nat :=
+    max_nats
+      (map (max_special_path_from vertices edge special fuel) vertices).
+
+  Lemma path_of_lengthb_sound :
+    forall vertices edge n x y,
+      path_of_lengthb vertices edge n x y = true ->
+      walk edge x y.
+  Proof.
+    intros vertices edge n.
+    induction n as [| n IH]; intros x y H.
+    - simpl in H.
+      apply eqb_sound in H. subst. constructor.
+    - simpl in H.
+      apply existsb_exists in H as [z [_ Hz]].
+      apply andb_true_iff in Hz as [Hedge Hpath].
+      eapply Walk_step.
+      + exact Hedge.
+      + now apply IH.
+  Qed.
+
+  Lemma successors_sound :
+    forall vertices edge x y,
+      In y (successors vertices edge x) ->
+      edge x y = true.
+  Proof.
+    intros vertices edge x y H.
+    unfold successors in H.
+    apply filter_In in H as [_ Hedge].
+    exact Hedge.
+  Qed.
+
+  Lemma add_fresh_In :
+    forall xs seen todo y,
+      In y (add_fresh xs seen todo) ->
+      In y todo \/ In y xs.
+  Proof.
+    induction xs as [| x xs IH]; intros seen todo y H; simpl in H.
+    - left. exact H.
+    - apply IH in H as [Htodo | Hxs].
+      + destruct (inb x seen || inb x todo) eqn:Halready.
+        * left. exact Htodo.
+        * simpl in Htodo.
+          destruct Htodo as [Hy | Hy].
+          -- subst. right. left. reflexivity.
+          -- left. exact Hy.
+      + right. right. exact Hxs.
+  Qed.
+
+  Lemma dfs_sound_from :
+    forall vertices edge fuel seen todo target source,
+      (forall z, In z todo -> walk edge source z) ->
+      dfs vertices edge fuel seen todo target = true ->
+      walk edge source target.
+  Proof.
+    intros vertices edge fuel.
+    induction fuel as [| fuel IH]; intros seen todo target source Htodo Hdfs.
+    - discriminate.
+    - destruct todo as [| x todo']; simpl in Hdfs; try discriminate.
+      destruct (inb x seen) eqn:Hseen.
+      + apply IH with (seen := seen) (todo := todo').
+        * intros z Hz. apply Htodo. simpl. auto.
+        * exact Hdfs.
+      + destruct (eqb x target) eqn:Htarget.
+        * apply eqb_sound in Htarget. subst.
+          apply Htodo. simpl. auto.
+        * apply IH with
+            (seen := x :: seen)
+            (todo := add_fresh (successors vertices edge x) (x :: seen) todo').
+          -- intros z Hz.
+             apply add_fresh_In in Hz as [Hz | Hz].
+             ++ apply Htodo. simpl. auto.
+             ++ eapply walk_trans.
+                ** apply Htodo. simpl. auto.
+                ** eapply Walk_step.
+                   --- apply successors_sound in Hz. exact Hz.
+                   --- constructor.
+          -- exact Hdfs.
+  Qed.
+
+  Lemma reachb_sound :
+    forall vertices edge fuel x y,
+      reachb vertices edge fuel x y = true ->
+      walk edge x y.
+  Proof.
+    intros vertices edge fuel x y H.
+    unfold reachb in H.
+    eapply dfs_sound_from; eauto.
+    intros z Hz.
+    simpl in Hz.
+    destruct Hz as [Hz | []].
+    subst. constructor.
+  Qed.
+
+  Lemma connectedb_sound :
+    forall vertices edge fuel x y,
+      connectedb vertices edge fuel x y = true ->
+      walk edge x y /\ walk edge y x.
+  Proof.
+    intros vertices edge fuel x y H.
+    unfold connectedb in H.
+    apply andb_true_iff in H as [Hxy Hyx].
+    split.
+    - eapply reachb_sound; eauto.
+    - eapply reachb_sound; eauto.
+  Qed.
+End GraphAlgorithms.
